Proof of model_E1E2_orutt_strict sound (with admitted lemmas like PickUnique).
File almost compiles now, but the LangRefine module changed to add
module parameters about safely converting addresses and
intptrs... This doesn't hold for the FinInfLangRefine module from
before. Not sure if it's needed yet, though.

src/coq/Semantics/InfiniteToFinite.v
@@ -5025,7 +5025,7 @@ Module Type LangRefine (IS1 : InterpreterStack) (IS2 : InterpreterStack) (AC1 : 
       dvalue_refine_lazy
       t1 t2.
 
-  Definition L0_E1E2_rutt_strict t1 t2
+  Definition L0_E1E2_orutt_strict t1 t2
     : Prop :=
     orutt
       event_refine_strict
@@ -5033,8 +5033,8 @@ Module Type LangRefine (IS1 : InterpreterStack) (IS2 : InterpreterStack) (AC1 : 
       dvalue_refine_strict
       t1 t2 (OOM:=OOME).
 
-  Definition model_E1E2_rutt_strict p1 p2 :=
-    L0_E1E2_rutt_strict
+  Definition model_E1E2_orutt_strict p1 p2 :=
+    L0_E1E2_orutt_strict
       (LLVM1.denote_vellvm (DTYPE_I 32%N) "main" LLVM1.main_args (convert_types (mcfg_of_tle p1)))
       (LLVM2.denote_vellvm (DTYPE_I 32%N) "main" LLVM2.main_args (convert_types (mcfg_of_tle p2))).
 
@@ -11837,14 +11837,14 @@ Module Type LangRefine (IS1 : InterpreterStack) (IS2 : InterpreterStack) (AC1 : 
     }
   Admitted.
 
-  (* Lemma uvalue_refine_concretize_poison : *)
-  (*   forall uv1 uv2, *)
-  (*     uvalue_refine uv1 uv2 -> *)
-  (*     (forall dt : dtyp, ~ IS1.LLVM.MEM.CP.CONC.concretize uv1 (IS1.LP.Events.DV.DVALUE_Poison dt)) <-> *)
-  (*       (forall dt : dtyp, ~ concretize uv2 (DVALUE_Poison dt)). *)
-  (* Proof. *)
-  (*   (* This may not be true if uv2 can OOM... *) *)
-  (* Admitted. *)
+  Lemma uvalue_refine_strict_concretize_poison :
+    forall uv1 uv2,
+      uvalue_refine_strict uv1 uv2 ->
+      (forall dt : dtyp, ~ IS1.LLVM.MEM.CP.CONC.concretize uv1 (IS1.LP.Events.DV.DVALUE_Poison dt)) <->
+        (forall dt : dtyp, ~ concretize uv2 (DVALUE_Poison dt)).
+  Proof.
+    (* This may not be true if uv2 can OOM... *)
+  Admitted.
 
   Lemma denote_mcfg_E1E2_orutt' :
     forall dfns1 dfns2 dt f1 f2 args1 args2,
@@ -12040,63 +12040,66 @@ Module Type LangRefine (IS1 : InterpreterStack) (IS2 : InterpreterStack) (AC1 : 
     split; auto.
   Qed.
 
-  Lemma model_E1E2_rutt_strict_sound
+  Lemma model_E1E2_orutt_strict_sound
     (p : list
            (LLVMAst.toplevel_entity
               LLVMAst.typ
               (LLVMAst.block LLVMAst.typ * list (LLVMAst.block LLVMAst.typ)))) :
-    model_E1E2_rutt p p.
+    model_E1E2_orutt_strict p p.
   Proof.
     red.
 
     unfold denote_vellvm.
     unfold LLVM1.denote_vellvm.
-    eapply rutt_bind; [apply build_global_environment_E1E2_rutt_strict_sound|].
+    eapply orutt_bind; [apply build_global_environment_E1E2_orutt_strict_sound|].
 
     intros [] [] _.
-    eapply rutt_bind; [apply address_one_functions_E1E2_rutt|].
+    eapply orutt_bind;
+      [apply rutt_orutt;
+       [apply address_one_functions_E1E2_rutt | solve_dec_oom]|].
 
     intros r1 r2 R1R2.
-    eapply rutt_bind; [apply GlobalRead_L0_E1E2_rutt|].
+    eapply orutt_bind;
+      [apply rutt_orutt;
+       [apply GlobalRead_L0_E1E2_rutt | solve_dec_oom]|].
 
     intros r3 r4 R3R4.
-    eapply rutt_bind.
+    eapply orutt_bind.
 
-    { apply denote_mcfg_E1E2_rutt; auto.
-      - apply dvalue_refine_dvalue_to_uvalue; auto.
+    { apply denote_mcfg_E1E2_orutt; auto.
+      - apply dvalue_refine_strict_dvalue_to_uvalue; auto.
       - (* TODO: fold into main_args lemma probably *)
         unfold main_args.
         unfold LLVM1.main_args.
         constructor.
-        + red.
-          rewrite uvalue_convert_equation.
+        + unfold_uvalue_refine_strict_goal.
           reflexivity.
         + constructor; [|constructor].
-          red.
-          rewrite uvalue_convert_equation.
+          unfold_uvalue_refine_strict_goal.
           cbn.
           rewrite AC1.addr_convert_null.
           reflexivity.
     }
 
     intros r0 r5 H.
-    eapply rutt_bind with (RR:=fun x y => dvalue_refine (proj1_sig x) (proj1_sig y)).
+    eapply orutt_bind with (RR:=fun x y => dvalue_refine_strict (proj1_sig x) (proj1_sig y)).
     { (* Pick *)
-      apply rutt_trigger.
+      apply orutt_trigger.
       { cbn.
         split; auto.
         (* TODO: this lemma may not even be true *)
-        apply uvalue_refine_concretize_poison; auto.
+        apply uvalue_refine_strict_concretize_poison; auto.
       }
 
       intros t1 t2 H0.
       cbn in *.
       destruct t1, t2; tauto.
+      intros o CONTRA; inv CONTRA.
     }
 
     intros r6 r7 H0.
     cbn.
-    apply rutt_Ret; auto.
+    apply orutt_Ret; auto.
   Qed.
 
   (* TODO: not sure about name... *)
@@ -12106,7 +12109,7 @@ Module Type LangRefine (IS1 : InterpreterStack) (IS2 : InterpreterStack) (AC1 : 
                            LLVMAst.typ
                            (LLVMAst.block LLVMAst.typ * list (LLVMAst.block LLVMAst.typ))))
     : Prop :=
-    refine_E1E2_L0
+    refine_E1E2_L0_strict
       (LLVM1.denote_vellvm (DTYPE_I 32%N) "main" LLVM1.main_args (convert_types (mcfg_of_tle p1)))
       (LLVM2.denote_vellvm (DTYPE_I 32%N) "main" LLVM2.main_args (convert_types (mcfg_of_tle p2))).
 
@@ -12117,7 +12120,7 @@ Module Type LangRefine (IS1 : InterpreterStack) (IS2 : InterpreterStack) (AC1 : 
                            LLVMAst.typ
                            (LLVMAst.block LLVMAst.typ * list (LLVMAst.block LLVMAst.typ))))
     : Prop :=
-    refine_E1E2_L1
+    refine_E1E2_L1_strict
       (LLVM1.model_oom_L1 p1)
       (LLVM2.model_oom_L1 p2).
 
@@ -12128,7 +12131,7 @@ Module Type LangRefine (IS1 : InterpreterStack) (IS2 : InterpreterStack) (AC1 : 
                            LLVMAst.typ
                            (LLVMAst.block LLVMAst.typ * list (LLVMAst.block LLVMAst.typ))))
     : Prop :=
-    refine_E1E2_L2
+    refine_E1E2_L2_strict
       (LLVM1.model_oom_L2 p1)
       (LLVM2.model_oom_L2 p2).
 
@@ -12139,7 +12142,7 @@ Module Type LangRefine (IS1 : InterpreterStack) (IS2 : InterpreterStack) (AC1 : 
                            LLVMAst.typ
                            (LLVMAst.block LLVMAst.typ * list (LLVMAst.block LLVMAst.typ))))
     : Prop :=
-    refine_E1E2_L3
+    refine_E1E2_L3_strict
       (LLVM1.model_oom_L3 p1)
       (LLVM2.model_oom_L3 p2).
 
@@ -12150,7 +12153,7 @@ Module Type LangRefine (IS1 : InterpreterStack) (IS2 : InterpreterStack) (AC1 : 
                            LLVMAst.typ
                            (LLVMAst.block LLVMAst.typ * list (LLVMAst.block LLVMAst.typ))))
     : Prop :=
-    refine_E1E2_L4 (LLVM1.model_oom_L4 p1) (LLVM2.model_oom_L4 p2).
+    refine_E1E2_L4_strict (LLVM1.model_oom_L4 p1) (LLVM2.model_oom_L4 p2).
 
   (* TODO: not sure about name... *)
   Definition model_E1E2_L5
@@ -12159,7 +12162,7 @@ Module Type LangRefine (IS1 : InterpreterStack) (IS2 : InterpreterStack) (AC1 : 
                            LLVMAst.typ
                            (LLVMAst.block LLVMAst.typ * list (LLVMAst.block LLVMAst.typ))))
     : Prop :=
-    refine_E1E2_L5 (LLVM1.model_oom_L5 p1) (LLVM2.model_oom_L5 p2).
+    refine_E1E2_L5_strict (LLVM1.model_oom_L5 p1) (LLVM2.model_oom_L5 p2).
 
   (* TODO: not sure about name... *)
   Definition model_E1E2_L6
@@ -12168,21 +12171,21 @@ Module Type LangRefine (IS1 : InterpreterStack) (IS2 : InterpreterStack) (AC1 : 
                            LLVMAst.typ
                            (LLVMAst.block LLVMAst.typ * list (LLVMAst.block LLVMAst.typ))))
     : Prop :=
-    refine_E1E2_L6 (LLVM1.model_oom_L6 p1) (LLVM2.model_oom_L6 p2).
+    refine_E1E2_L6_strict (LLVM1.model_oom_L6 p1) (LLVM2.model_oom_L6 p2).
 
 End LangRefine.
 
-Module MakeLangRefine (IS1 : InterpreterStack) (IS2 : InterpreterStack) (AC1 : AddrConvert IS1.LP.ADDR IS2.LP.ADDR) (AC2 : AddrConvert IS2.LP.ADDR IS1.LP.ADDR) (LLVM1 : LLVMTopLevel IS1) (LLVM2 : LLVMTopLevel IS2) (TLR : TopLevelRefinements IS2 LLVM2) : LangRefine IS1 IS2 AC1 AC2 LLVM1 LLVM2 TLR.
-  Include LangRefine IS1 IS2 AC1 AC2 LLVM1 LLVM2 TLR.
+Module MakeLangRefine (IS1 : InterpreterStack) (IS2 : InterpreterStack) (AC1 : AddrConvert IS1.LP.ADDR IS2.LP.ADDR) (AC2 : AddrConvert IS2.LP.ADDR IS1.LP.ADDR) (LLVM1 : LLVMTopLevel IS1) (LLVM2 : LLVMTopLevel IS2) (TLR : TopLevelRefinements IS2 LLVM2) (ACS : AddrConvertSafe IS2.LP.ADDR IS1.LP.ADDR AC2 AC1) (IPS : IPConvertSafe IS2.LP.IP IS1.LP.IP) : LangRefine IS1 IS2 AC1 AC2 LLVM1 LLVM2 TLR ACS IPS.
+  Include LangRefine IS1 IS2 AC1 AC2 LLVM1 LLVM2 TLR ACS IPS.
 End MakeLangRefine.
 
-Module InfFinLangRefine := MakeLangRefine InterpreterStackBigIntptr InterpreterStack64BitIntptr InfToFinAddrConvert FinToInfAddrConvert TopLevelBigIntptr TopLevel64BitIntptr TopLevelRefinements64BitIntptr.
+Module InfFinLangRefine := MakeLangRefine InterpreterStackBigIntptr InterpreterStack64BitIntptr InfToFinAddrConvert FinToInfAddrConvert TopLevelBigIntptr TopLevel64BitIntptr TopLevelRefinements64BitIntptr FinToInfAddrConvertSafe FinToInfIntptrConvertSafe.
 
 (* Just planning on using this for L4_convert from finite to infinite events. *)
-Module FinInfLangRefine := MakeLangRefine InterpreterStack64BitIntptr InterpreterStackBigIntptr FinToInfAddrConvert InfToFinAddrConvert TopLevel64BitIntptr TopLevelBigIntptr TopLevelRefinementsBigIntptr.
+(* Module FinInfLangRefine := MakeLangRefine InterpreterStack64BitIntptr InterpreterStackBigIntptr FinToInfAddrConvert InfToFinAddrConvert TopLevel64BitIntptr TopLevelBigIntptr TopLevelRefinementsBigIntptr FinToInfAddrConvertSafe FinToInfIntptrConvertSafe. *)
 
 Module InfiniteToFinite.
-  Import FinInfLangRefine. (* Just planning on using this for L4_convert from finite to infinite events. *)
+  (* Import FinInfLangRefine. (* Just planning on using this for L4_convert from finite to infinite events. *) *)
   Import InfFinLangRefine.
 
   From Vellvm Require Import InterpreterMCFG.
@@ -12207,10 +12210,10 @@ Module InfiniteToFinite.
   Module InfLLVM := Vellvm.Semantics.InterpretationStack.InterpreterStackBigIntptr.LLVM.
   Module FinLLVM := Vellvm.Semantics.InterpretationStack.InterpreterStack64BitIntptr.LLVM.
   Module InfFinTC := Vellvm.Semantics.InfiniteToFinite.InfFinLangRefine.TC1.
-  Module FinInfTC := Vellvm.Semantics.InfiniteToFinite.FinInfLangRefine.TC1.
+  (* Module FinInfTC := Vellvm.Semantics.InfiniteToFinite.FinInfLangRefine.TC1. *)
 
   Module EC1 := InfFinTC.EC.
-  Module EC2 := FinInfTC.EC.
+  (* Module EC2 := FinInfTC.EC. *)
 
   Module InfMem := MemoryBigIntptr.
   Module FinMem := Memory64BitIntptr.
